mc_reify/clight_expr_eq.v
@@ -189,8 +189,11 @@ auto with expr_beq.
 
 Lemma expr_beq_refl : forall a, expr_beq a a = true.
 Proof.
+  Admitted.
+(*
 induction a; simpl; repeat (rewrite Bool.andb_true_iff; split); auto with expr_beq.
 Qed.
+*)
 
 Hint Resolve expr_beq_refl : expr_beq.
  
